Software/Doc/Example/Verification/System1/Package/NatRangeIterator.v
@@ -10,13 +10,60 @@ Import ObjectOrientedNotations.
 Open Scope oo_scope.
 Open Scope exec_scope.
 
-Lemma get_at_start :
+Lemma proof_get_at_start :
   get_at_start exec_step.
 Proof.
   unfold get_at_start. intros.
-  unfold wf_fun in H. destruct H. subst x.
-  Time reduce_clos_refl_trans_term.
-  Abort.
+  unfold wf_fun in H.
+  destruct H. destruct H0. subst x.
+  destruct st as [sk rpsk sr].
+  simpl in H1.
+  (* Rule out empty stack *)
+  destruct sk as [| sf sk].
+  { exfalso. apply H1. reflexivity. }
+  reduce_clos_refl_trans_term.
+  eapply Relation_Operators.rt1n_trans.
+    reduce_tcall.
+    reduce_value.
+    reduce_value.
+    reduce_value.
+  simpl.
+  eapply Relation_Operators.rt1n_trans.
+    reduce_treturn.
+    reduce_exec_step.
+    reduce_called_on_class.
+  simpl.
+  eapply Relation_Operators.rt1n_trans.
+    reduce_treturn.
+    reduce_tfield_r.
+    reduce_tvar.
+  simpl.
+  eapply Relation_Operators.rt1n_trans.
+    reduce_treturn.
+    reduce_tfield_r.
+    reduce_read_store.
+  simpl.
+  eapply Relation_Operators.rt1n_trans.
+    reduce_treturn.
+    reduce_value.
+  simpl.
+  apply Relation_Operators.rt1n_refl.
+  Qed.
+
+Lemma proof_get_at_start' :
+  get_at_start exec_step.
+Proof.
+  unfold NatRangeIterator.get_at_start. intros.
+    unfold wf_fun in H.
+  destruct H. destruct H0. subst x.
+  destruct st as [sk rpsk sr].
+  simpl in H1.
+  (* Rule out empty stack *)
+  destruct sk as [| sf sk].
+  { exfalso. apply H1. reflexivity. }
+  reduce_clos_refl_trans_term.
+  repeat reduce.
+  Qed.
 
 Close Scope exec_scope.
 Close Scope oo_scope.
